\documentclass[../../../main.tex]{subfiles}
\begin{document}
Particle under harmonic potential is subjected to the potential in the following form
\begin{equation*}
    V(x) = \frac{1}{2} m \omega^{2} x^{2},
\end{equation*}
In the $X$ basis, the Schrödinger equation now reads
\begin{equation*}
    -\frac{\hbar^{2}}{2m} \frac{d^{2}\psi(x)}{dx^{2}} + \frac{1}{2}m\omega^{2}x^{2}\psi(x) = E\psi(x).
\end{equation*}
Solving this yields discrete energy eigenvalues
\[
    E_{n} = \hbar\omega \left(n + \frac{1}{2}\right), \quad n = 0, 1, 2, \ldots
\]
and normalized eigenfunctions
\[
    \psi_{n}(x) = \left(\frac{m\omega}{\pi\hbar}\right)^{1/4} \frac{1}{\sqrt{2^{n} n!}} H_{n}\left(\sqrt{\frac{m\omega}{\hbar}} x\right) e^{-\frac{m\omega x^{2}}{2\hbar}}
\]
where \(H_{n}\) are Hermite polynomials.
Here are the first few.
\begin{align*}
    H_{0}(x) & = 1,                     \\
    H_{1}(x) & = 2x,                    \\
    H_{2}(x) & = 4x^{2} - 2,            \\
    H_{3}(x) & = 8x^{3} - 12x,          \\
    H_{4}(x) & = 16x^{4} - 48x^{2} + 12
\end{align*}

\subsection{Derivation}
From the Schrödinger equation
\begin{equation*}
    \frac{d^{2}\psi(x)}{dx^{2}} + \frac{2m }{\hbar^2 }\left(E-\omega^{2}x^{2}\right)\psi(x)
\end{equation*}
we make the substitution of $x=by$, which result in differential
\begin{align*}
    \frac{d\psi }{dx}       & =\frac{d\psi }{dy}\frac{dy }{dx}=\frac{1 }{b }\frac{d\psi }{dy}                                                                       \\
    \frac{d^2 \psi }{dx^2 } & = \frac{d }{dx }\left( \frac{1 }{b }\frac{d\psi }{dy} \right) =\frac{1 }{b}\frac{d^2\psi }{dy\;dx}=\frac{1 }{b }\frac{d^2\psi }{dy^2}
\end{align*}
Now Schrödinger equation reads
\begin{equation*}
    \frac{1 }{b^2 }\frac{d^2\psi }{dy^2 }+\frac{2m }{\hbar^2 }\left( E-\frac{1 }{2 }m\omega^2b^2y^2   \right) \psi=0
\end{equation*}
or
\begin{equation*}
    \frac{d^2\psi }{dy^2 }+\left( \frac{2mEb^2 }{\hbar^2 }-\frac{m^2\omega^2b^4y^2 }{\hbar^2}   \right) \psi=0
\end{equation*}
Now define
\begin{equation*}
    \epsilon=\frac{mEb^2 }{\hbar^2}=\frac{E }{\hbar\omega},\qquad b^2=\frac{\hbar }{m\omega}
\end{equation*}
Then
\begin{equation*}
    \frac{d^2 \psi}{dy^2}+(2\epsilon-y^2)\psi=0
\end{equation*}
Compare this to the Hermite equation
\begin{equation*}
    y_n''+(2n+1-x^2)y_n=0
\end{equation*}
which has the solution called the Hermite function
\begin{equation*}
    y_n=e^{x^2/2}\left(\frac{d}{dx}\right)^ne^{-x^2}=e^{-x^2/2}H_n(x)
\end{equation*}
On comparing $2\epsilon$ with $2n+1$, we obtain the expression for energy.
Then the solution to the Schrödinger equation is
\begin{equation*}
    \psi(y)=e^{-y^2/2}H_n(y)\qquad\text{or}\qquad\psi(x)=\exp \left[ -\frac{m\omega }{2 \hbar}x^2 \right] H_n \left[ \left( \frac{m \omega }{\hbar }^{1/2}x \right)  \right]
\end{equation*}

All that left is normalization.
To do so consider the orthogonality of Hermite polynomials
\begin{equation*}
    \int_{-\infty}^{\infty}e^{-x^2}H_n(x)H_m(x)\;dx=\sqrt{\pi}2^n n!\delta_{nm}
\end{equation*}
Therefore
\begin{align*}
    \int \psi ^*(x )\psi(x)\;dx=\int A^2\exp \left[ -\frac{m\omega }{ \hbar}x^2 \right] H_n \left\{\left[ \left( \frac{m \omega }{\hbar }^{1/2}x \right)  \right] \right\}^2\;dx                                                                            \\
      & = A^2 \left( \frac{\hbar }{m\omega} \right)^{1/2} \int\int A^2\exp \left[ -\frac{m\omega }{ \hbar}x^2 \right] H_n \left\{\left[ \left( \frac{m \omega }{\hbar }^{1/2}x \right)  \right] \right\}^2\;d \left( \sqrt{\frac{m\omega }{\hbar}x} \right) \\
    1 & = A^2  \sqrt{\frac{\hbar }{m\omega }}(\pi)^{1/2}2^nn!                                                                                                                                                                                               \\
    A=\left( \frac{m\omega }{\pi \hbar 2^{2n}(n!)^2 } \right) ^{1/4}
\end{align*}
Inserting this into the wavefunction yields the normalized wavefunction.
\end{document}